\documentclass[12]{article}
\usepackage[margin = 1in]{geometry}
\usepackage{amsmath}
\usepackage{listings}
\begin{document}

\title{Nondimensionalization}
\author{Abraham Teklu}
\date{}
\maketitle
When we start with the equation for the the rate of change of a population:
$$\frac{dP}{dt} = PN(P)$$
Where $N(P)$ is a function of population, and $P$ is the population. If we say $N(P)$ is the following:
$$N(P) = \pm a$$
Where a is constant and the sign depends on whether the population is growing or shrinking. 
\\
But this isn't accurate. The larger the population the more competition which will cause the competition; this can be represented more accurately with the following equation:
$$\frac{dP}{dt} = P(a-a'P)$$ 
Where $a$ and $a'$ are corresponding units to make the entire equation population per time. To nondimensionalize this equation we can turn it into the following form:
$$\frac{d\bar{P}}{d\bar{t}} = \bar{P}(1-\bar{P})$$ 
Where $\bar{P} = \frac{P}{P_{ref}}$ and $\bar{t} = \frac{t}{t_{ref}}$. Where $P_{ref}$ and $t_{ref}$ are reference times and populations. We can do this like the following:
$$d\bar{P} = \frac{dP}{P_{ref}}~~~~ d\bar{t} = \frac{dt}{t_{ref}} \rightarrow \bar{dP}P_{ref} = dP ~~~~ \bar{t}t_{ref} = t$$
If we plug this in to dimensional equation:
$$\frac{d\bar{P}}{d\bar{t}} \frac{P_{ref}}{t_{ref}} = \bar{P}P_{ref}(a-a'\bar{P}P_{ref})$$
$$\frac{d\bar{P}}{d\bar{t}} = \bar{P}t_{ref}a-a'\bar{P}^2P_{ref}t_{ref}$$
So we can conclude:
$$t_{ref}a = 1 ~~~~~ P_{ref}t_{ref}a' = 1$$
and then
$$t_{ref} = \frac{1}{a} ~~~~~~~ P_{ref} = \frac{a}{a'}$$
\end{document}